Henret/Proofs.lean
@@ -9,6 +9,8 @@ import Henret.Proofs.InvariantsPreservation
 import Henret.Proofs.ResourceReachable
 import Henret.Proofs.ResourceBranch
 import Henret.Proofs.Policy
+import Henret.Proofs.Metadata
+import Henret.Proofs.MetaPolicy
 import Henret.Proofs.Parenthood
 import Henret.Proofs.Occurrence
 import Henret.Proofs.Supervision
